Exposing mgf_hash

code/rsapss/Hacl.RSAPSS.fst
@@ -84,3 +84,9 @@ val rsapss_pkey_verify:
 let rsapss_pkey_verify a modBits eBits nb eb saltLen sgntLen sgnt msgLen msg =
   RI.rsapss_pkey_verify (ke modBits) a modBits
     (load_pkey modBits) (rsapss_verify a modBits) eBits nb eb saltLen sgntLen sgnt msgLen msg
+
+[@ (Comment "Miscellaneous functions")]
+
+val mgf_hash: a:Hash.algorithm{S.hash_is_supported a} -> Hacl.Impl.RSAPSS.MGF.mgf_hash_st a
+
+let mgf_hash a len mgfseed maskLen res = Hacl.Impl.RSAPSS.MGF.mgf_hash a len mgfseed maskLen res
